Adapt to latest metacoq

theories/LambdaBoxMut/compile.v
@@ -336,7 +336,7 @@ Fixpoint list_Defs (l : list (def Term)) : Defs :=
   | t :: ts => dcons t.(dname) t.(dbody) t.(rarg) (list_Defs ts) 
   end.
 
-Equations trans_prim_val {T} (p : EPrimitive.prim_val T) : option primitive :=
+Polymorphic Equations trans_prim_val {T} (p : EPrimitive.prim_val T) : option primitive :=
   trans_prim_val (existT _ primInt (primIntModel i)) => Some (existT _ AstCommon.primInt i) ;
   trans_prim_val (existT _ primFloat (primFloatModel i)) => Some (existT _ AstCommon.primFloat i) ;
   trans_prim_val (existT _ primArray _) => None.
