theories/Codegen/LambdaANF_to_Clight_stack.v
@@ -799,8 +799,8 @@ Definition compile_float (cenv : ctor_env) (ienv : n_ind_env) (fenv : fun_env) (
 
 Definition compile_primitive (cenv : ctor_env) (ienv : n_ind_env) (fenv : fun_env) (map : fun_info_env) (x : positive) (p : AstCommon.primitive) : statement :=
   match projT1 p as tag return AstCommon.prim_value tag -> statement with
-  | Primitive.primInt => fun i => x ::= Econst_long (to_int64 i) (Tlong Unsigned noattr)
-  | Primitive.primFloat => fun f => compile_float cenv ienv fenv map x (to_float f)
+  | AstCommon.primInt => fun i => x ::= Econst_long (to_int64 i) (Tlong Unsigned noattr)
+  | AstCommon.primFloat => fun f => compile_float cenv ienv fenv map x (to_float f)
   end (projT2 p).
 
 Section Translation.
